[vfa] finish Binom

vfa-1.5.4/Binom.v
@@ -180,32 +180,107 @@ Definition priq (q: priqueue) : Prop := priq' 0 q.
 
 (** **** Exercise: 1 star, standard (empty_priq)  *)
 Theorem empty_priq: priq empty.
-(* FILL IN HERE *) Admitted.
+Proof.
+  unfold priq,priq'. simpl. exact I.
+Qed.
 (** [] *)
 
 (** **** Exercise: 2 stars, standard (smash_valid) *)
 Theorem smash_valid:
        forall n t u, pow2heap n t -> pow2heap n u -> pow2heap (S n) (smash t u).
-(* FILL IN HERE *) Admitted.
+Proof.
+  intros n t u Ht Hu. destruct t; simpl in *; [|contradiction].
+  destruct u; simpl in *; [|contradiction].
+  destruct t2; simpl in *; [contradiction|].
+  destruct u2; simpl in *; [contradiction|].
+  bdestruct (k >? k0); simpl.
+  - refine (conj _ (conj Hu Ht)). lia.
+  - refine (conj H (conj Ht Hu)).
+Qed.
 (** [] *)
 
 (** **** Exercise: 3 stars, standard (carry_valid) *)
 Theorem carry_valid:
            forall n q,  priq' n q ->
            forall t, (t=Leaf \/ pow2heap n t) -> priq' n (carry q t).
-(* FILL IN HERE *) Admitted.
+Proof.
+  intros n q. generalize dependent n.
+  induction q; intros n H t Ht.
+  - destruct t.
+    + destruct Ht as [Ht | Ht]; [discriminate Ht|].
+      simpl in *. exact (conj (or_intror Ht) I).
+    + simpl. exact I.
+  - simpl in *. destruct H as [H Hpq].
+    destruct a.
+    + destruct H; [discriminate H|]. simpl in *.
+      destruct a2; simpl in *; [contradiction|].
+      destruct t.
+      * destruct Ht as [Ht | Ht]; [discriminate Ht|].
+        cbn delta [priq'] fix. cbn iota.
+        refine (conj (or_introl eq_refl) _).
+        apply (IHq _ Hpq).
+        right. apply (smash_valid _ _ _ Ht).
+        simpl. assumption.
+      * simpl. exact (conj (or_intror H) Hpq).
+    + simpl. exact (conj Ht Hpq).
+Qed.
 (** [] *)
 
 (** **** Exercise: 2 stars, standard, optional (insert_valid) *)
 Theorem insert_priq: forall x q, priq q -> priq (insert x q).
-(* FILL IN HERE *) Admitted.
+Proof.
+  intros x q H. unfold priq in *.
+  apply carry_valid.
+  - apply H.
+  - right. simpl. exact I.
+Qed.
 (** [] *)
 
 (** **** Exercise: 3 stars, standard, optional (join_valid) *)
 (* This proof is rather long, but each step is reasonably straightforward.
     There's just one [induction] to do, right at the beginning. *)
 Theorem join_valid: forall p q c n, priq' n p -> priq' n q -> (c=Leaf \/ pow2heap n c) -> priq' n (join p q c).
-(* FILL IN HERE *) Admitted.
+Proof.
+  induction p; intros q c n Hp Hq Hc; simpl.
+  - apply carry_valid; assumption.
+  - simpl in Hp. destruct Hp as [Ha Hp].
+    destruct a; simpl in Ha.
+    + destruct Ha as [Ha | Ha]; [discriminate Ha|].
+      destruct a2; [contradiction|].
+      destruct q.
+      * destruct c.
+          { destruct Hc as [Hc | Hc]; [discriminate Hc|].
+            cbn delta [priq'] fix. cbn iota.
+            refine (conj (or_introl eq_refl) _).
+            apply (carry_valid _ _ Hp). right.
+            apply (smash_valid _ _ _ Hc). simpl. exact Ha. }
+          { simpl. exact (conj (or_intror Ha) Hp). }
+      * simpl in Hq. destruct Hq as [Ht Hq].
+        destruct t.
+          { destruct Ht as [Ht | Ht]; [discriminate Ht|].
+            cbn delta [priq'] fix. cbn iota.
+            refine (conj Hc _). apply (IHp _ _ _ Hp Hq).
+            right. refine (smash_valid _ _ _ _ Ht).
+            simpl. exact Ha. }
+          { destruct c; cbn delta [priq'] fix; cbn iota.
+            - destruct Hc as [Hc | Hc]; [discriminate Hc|].
+              refine (conj Ht (IHp _ _ _ Hp Hq (or_intror _))).
+              apply (smash_valid _ _ _ Hc). simpl. assumption.
+            - refine (conj (or_intror _) (IHp _ _ _ Hp Hq (or_introl eq_refl))).
+              simpl. apply Ha. }
+    + destruct q.
+      * simpl. exact (conj Hc Hp).
+      * simpl in Hq. destruct Hq as [Ht Hq].
+        destruct t.
+          { destruct Ht as [Ht | Ht]; [discriminate Ht|].
+            destruct c; cbn delta [priq'] fix; cbn iota.
+            - destruct Hc as [Hc | Hc]; [discriminate Hc|].
+              refine (conj (or_introl eq_refl) (IHp _ _ _ Hp Hq (or_intror _))).
+              exact (smash_valid _ _ _ Hc Ht).
+            - cbn delta [priq'] fix. cbn iota.
+              exact (conj (or_intror Ht) (IHp _ _ _ Hp Hq (or_introl eq_refl))). }
+          { exact (conj Hc (IHp _ _ _ Hp Hq (or_introl eq_refl))). }
+Qed.
 (** [] *)
 
 Theorem merge_priq:  forall p q, priq p -> priq q -> priq (merge p q).
@@ -213,10 +288,70 @@ Proof.
  intros. unfold merge. apply join_valid; auto.
 Qed.
 
+Lemma unzip_valid : forall t cont n m, pow2heap' n m t ->
+  priq' n (cont nil) ->
+  priq (unzip t cont).
+Proof.
+  induction t; intros cont n m Ht Hc.
+  - destruct n; [contradiction Ht|].
+    simpl in Ht. destruct Ht as [Hm [Ht1 Ht2]].
+    simpl.
+    apply (IHt2 _ _ _ Ht2). simpl.
+    exact (conj (or_intror Ht1) Hc).
+  - destruct n.
+    + exact Hc.
+    + contradiction Ht.
+Qed.
+
+Lemma heap_delete_max_priq : forall t n, pow2heap n t -> priq (heap_delete_max t).
+Proof.
+  refine (fun t => match t with
+          | Node _ t1 Leaf => _
+          | _ => fun _ _ => empty_priq
+          end).
+  clear t t0. simpl. intros n H.
+  apply (unzip_valid _ _ _ _ H). exact I.
+Qed.
+
+Lemma delete_max_aux_priq : forall k q n,
+  priq' n q ->
+  let (p0,p1) := delete_max_aux k q in priq' n p0 /\ priq p1.
+Proof.
+  intros k q. induction q; intros n Hq.
+  - simpl. exact (conj I I).
+  - cbn delta [delete_max_aux] fix. cbn iota.
+    destruct a as [ak al ar|].
+    + destruct ar as [ark arl arr|].
+      * simpl. exact (conj I I).
+      * simpl in Hq. destruct Hq as [Ha Hq].
+        bdestruct (k >? ak).
+          { destruct (delete_max_aux k q).
+            apply IHq in Hq. destruct Hq as [Hp Hp0].
+            simpl. exact (conj (conj Ha Hp) Hp0). }
+          { split.
+            - simpl. exact (conj (or_introl eq_refl) Hq).
+            - destruct Ha as [Ha | Ha]. { discriminate Ha. }
+              apply (heap_delete_max_priq _ n).
+              apply Ha. }
+    + destruct (delete_max_aux k q).
+      simpl in Hq. destruct Hq as [H Hq].
+      apply IHq in Hq. destruct Hq as [Hp Hp0].
+      simpl. exact (conj (conj H Hp) Hp0).
+Qed.          
+
 (** **** Exercise: 5 stars, standard, optional (delete_max_Some_priq) *)
 Theorem delete_max_Some_priq:
       forall p q k, priq p -> delete_max p = Some(k,q) -> priq q.
-(* FILL IN HERE *) Admitted.
+Proof.
+  unfold delete_max.
+  intros p q k Hp Ed.
+  destruct (find_max p); [| discriminate Ed].
+  apply (delete_max_aux_priq k0) in Hp. 
+  destruct (delete_max_aux k0 p).
+  injection Ed as Ek Eq. subst k q.
+  destruct Hp as [Hp0 Hp1].
+  exact (join_valid _ _ _ _ Hp0 Hp1 (or_introl eq_refl)).
+Qed.
 (** [] *)
 
 (* ================================================================= *)
@@ -245,7 +380,12 @@ Inductive tree_elems: tree -> list key -> Prop :=
 *)
 
 Inductive priqueue_elems: list tree -> list key -> Prop :=
-             (* FILL IN HERE *)
+  | priqueue_elems_nil : priqueue_elems [] []
+  | priqueue_elems_cons : forall ht hl tt tl l,
+      tree_elems ht hl ->
+      priqueue_elems tt tl ->
+      Permutation (hl ++ tl) l ->
+      priqueue_elems (ht :: tt) l
 .
 (* Do not modify the following line: *)
 Definition manual_grade_for_priqueue_elems : option (nat*string) := None.
@@ -262,13 +402,26 @@ Definition Abs (p: priqueue) (al: list key) := priqueue_elems p al.
 
 Theorem tree_elems_ext: forall t e1 e2,
   Permutation e1 e2 -> tree_elems t e1 -> tree_elems t e2.
-(* FILL IN HERE *) Admitted.
+Proof.
+  intros t e1 e2 Hp He. destruct He.
+  - apply Permutation_nil in Hp. subst e2. apply tree_elems_leaf.
+  - refine (tree_elems_node _ _ _ _ _ _ He1 He2 _).
+    apply Permutation_sym in Hp.
+    exact (perm_trans Hp H).
+Qed.
 (** [] *)
 
 (** **** Exercise: 2 stars, standard (tree_perm) *)
 Theorem tree_perm: forall t e1 e2,
   tree_elems t e1 -> tree_elems t e2 -> Permutation e1 e2.
-(* FILL IN HERE *) Admitted.
+Proof.
+  intros t e1 e2 He1. generalize dependent e2.
+  induction He1; intros e2 He2.
+  - inv He2. apply perm_nil.
+  - inv He2. apply Permutation_sym in H6.
+    refine (perm_trans H (perm_trans (perm_skip _ _) H6)).
+    exact (Permutation_app (IHHe1_1 _ H3) (IHHe1_2 _ H5)).
+Qed.
 (** [] *)
 
 (** **** Exercise: 2 stars, standard (priqueue_elems_ext)
@@ -278,24 +431,54 @@ Theorem tree_perm: forall t e1 e2,
 
 Theorem priqueue_elems_ext: forall q e1 e2,
   Permutation e1 e2 -> priqueue_elems q e1 -> priqueue_elems q e2.
-(* FILL IN HERE *) Admitted.
+Proof.
+  intros q e1 e2 Hp Hq. destruct Hq.
+  - apply Permutation_nil in Hp. subst e2. apply priqueue_elems_nil.
+  - refine (priqueue_elems_cons _ _ _ _ _ H Hq _).
+    apply (perm_trans H0 Hp).
+Qed.
 (** [] *)
+
+Lemma abs_perm': forall p al bl,
+   Abs p al -> Abs p bl -> Permutation al bl.
+Proof.
+  unfold Abs.
+  intros p al bl Ha. generalize dependent bl.
+  induction Ha; intros bl Hb.
+  - inv Hb. apply perm_nil.
+  - inv Hb. apply Permutation_sym in H0.
+    refine (perm_trans H0 (perm_trans _ H6)).
+    exact (Permutation_app (tree_perm _ _ _ H H3) (IHHa _ H4)).
+Qed.
 
 (** **** Exercise: 2 stars, standard (abs_perm) *)
 Theorem abs_perm: forall p al bl,
    priq p -> Abs p al -> Abs p bl -> Permutation al bl.
 Proof.
-(* FILL IN HERE *) Admitted.
+  exact (fun p al bl _ Hea Heb => abs_perm' p al bl Hea Heb).
+Qed.
 (** [] *)
 
 (** **** Exercise: 2 stars, standard (can_relate) *)
 Lemma tree_can_relate: forall t, exists al, tree_elems t al.
 Proof.
-(* FILL IN HERE *) Admitted.
+  induction t.
+  - destruct IHt1 as [ll Hl].
+    destruct IHt2 as [lr Hr].
+    exists (k :: ll++lr).
+    apply (tree_elems_node _ _ _ _ _ _ Hl Hr (Permutation_refl _)).
+  - exists []. apply tree_elems_leaf.
+Qed.
 
 Theorem can_relate:  forall p, priq p -> exists al, Abs p al.
 Proof.
-(* FILL IN HERE *) Admitted.
+  intros q _. induction q.
+  - exists []. apply priqueue_elems_nil.
+  - destruct IHq as [tl Ht].
+    destruct (tree_can_relate a) as [al Ha].
+    exists (al ++ tl).
+    apply (priqueue_elems_cons _ _ _ _ _ Ha Ht (Permutation_refl _)).
+Qed.
 (** [] *)
 
 (* ================================================================= *)
@@ -303,7 +486,8 @@ Proof.
 (** **** Exercise: 1 star, standard (empty_relate) *)
 Theorem empty_relate:  Abs empty nil.
 Proof.
-(* FILL IN HERE *) Admitted.
+  apply priqueue_elems_nil.
+Qed.
 (** [] *)
 
 (** **** Exercise: 3 stars, standard (smash_elems)
@@ -314,7 +498,28 @@ Theorem smash_elems: forall n t u bt bu,
                      pow2heap n t -> pow2heap n u ->
                      tree_elems t bt -> tree_elems u bu ->
                      tree_elems (smash t u) (bt ++ bu).
-(* FILL IN HERE *) Admitted.
+Proof.
+  intros n t u bt bu Hht Hhu Het Heu.
+  destruct t; [| contradiction Hht]. destruct u; [| contradiction Hhu].
+  simpl in *.
+  destruct t2; [contradiction Hht|]. destruct u2; [contradiction Hhu|].
+  inv Het. inv Heu.
+  inv H7. inv H4. rewrite app_nil_r in *.
+  bdestruct (k >? k0).
+  - refine (tree_elems_node _ _ _ _ _ _ _ tree_elems_leaf _).
+    + exact (tree_elems_node _ _ _ _ _ _ H3 H2 (Permutation_refl _)).
+    + rewrite app_nil_r.
+      refine (perm_trans (Permutation_app H5 H8) _). simpl.
+      apply perm_skip. apply Permutation_sym.
+      exact (Permutation_cons_app _ _ _ (Permutation_app_comm _ _)).
+  - refine (tree_elems_node _ _ _ _ _ _ _ tree_elems_leaf _).
+    + exact (tree_elems_node _ _ _ _ _ _ H2 H3 (Permutation_refl _)).
+    + rewrite app_nil_r.
+      refine (perm_trans (Permutation_app H5 H8) _). simpl.
+      change (k0 :: k :: bl ++ bl0) with ([k0] ++ (k :: bl ++ bl0)).
+      apply Permutation_cons_app. simpl.
+      apply Permutation_sym. apply Permutation_cons_app. apply Permutation_refl.
+Qed.
 (** [] *)
 
 (* ================================================================= *)
@@ -329,13 +534,48 @@ Theorem carry_elems:
       forall eq et, priqueue_elems q eq ->
                           tree_elems t et ->
                           priqueue_elems (carry q t) (eq++et).
-(* FILL IN HERE *) Admitted.
+Proof.
+  intros n q. generalize dependent n.
+  induction q; intros n Hpq t Hht eq et Heq Het.
+  - inv Heq. simpl. destruct t.
+    + refine (priqueue_elems_cons _ _ _ _ _ Het priqueue_elems_nil _).
+      rewrite app_nil_r. apply Permutation_refl.
+    + inv Het. apply priqueue_elems_nil.
+  - simpl in *.
+    destruct Hpq as [Hha Hpq]. inv Heq.
+    destruct a.
+    + destruct Hha as [Hha | Hha]; [discriminate Hha|].
+      destruct t.
+      * destruct Hht as [Hht | Hht]; [discriminate Hht|].
+        refine (priqueue_elems_cons _ _ _ (tl ++ (hl ++ et)) _ tree_elems_leaf _ _).
+          { refine (IHq _ Hpq _ (or_intror _) _ _ H2 _).
+            - apply smash_valid; assumption.
+            - refine (tree_elems_ext _ _ _ (Permutation_app_comm _ _) _).
+              exact (smash_elems _ _ _ _ _ Hht Hha Het H1). }
+          { simpl. rewrite app_assoc.
+            refine (Permutation_app _ (Permutation_refl _)).
+            refine (perm_trans (Permutation_app_comm _ _) H4). }
+      * inv Het. rewrite app_nil_r.
+        apply (priqueue_elems_cons _ _ _ _ _ H1 H2 H4).
+    + inv H1. simpl in H4.
+      apply (priqueue_elems_cons _ _ _ _ _ Het H2).
+      apply (perm_trans (Permutation_app_comm _ _)).
+      exact (Permutation_app H4 (Permutation_refl _)).
+Qed.
 (** [] *)
 
 (** **** Exercise: 2 stars, standard, optional (insert_elems) *)
 Theorem insert_relate:
         forall p al k, priq p -> Abs p al -> Abs (insert k p) (k::al).
-(* FILL IN HERE *) Admitted.
+Proof.
+  intros p al k Hpp Hep. unfold insert.
+  apply (priqueue_elems_ext _ (al ++ [k])).
+  - change (k :: al) with ([k] ++ al). apply Permutation_app_comm.
+  - apply (carry_elems _ _ Hpp).
+    + right. simpl. exact I.
+    + exact Hep.
+    + exact (tree_elems_node _ _ _ _ _ _ tree_elems_leaf tree_elems_leaf (Permutation_refl _)).
+Qed.
 (** [] *)
 
 (** **** Exercise: 4 stars, standard, optional (join_elems) *)
@@ -349,7 +589,91 @@ Theorem join_elems:
                              priqueue_elems q qe ->
                              tree_elems c ce ->
                               priqueue_elems (join p q c) (ce++pe++qe).
-(* FILL IN HERE *) Admitted.
+Proof.
+  induction p; intros q c n Hpp Hpq Hhc pe qe ce Hep Heq Hec.
+  - inv Hep. simpl.
+    refine (priqueue_elems_ext _ _ _ (Permutation_app_comm _ _) _).
+    apply (carry_elems _ _ Hpq); assumption.
+  - simpl. simpl in Hpp. destruct Hpp as [Hha Hpp].
+    destruct a as [ak al ar|].
+    + destruct Hha as [Hha | Hha]; [discriminate Hha|].
+      inv Hep.
+      destruct q.
+      * inv Heq. rewrite app_nil_r. destruct c.
+          { destruct Hhc as [Hhc | Hhc]; [discriminate Hhc|].
+            apply (priqueue_elems_cons _ _ _ (tl ++ (ce ++ hl)) _ tree_elems_leaf).
+            - apply (carry_elems _ _ Hpp).
+              + right. apply smash_valid; assumption.
+              + assumption.
+              + apply (smash_elems _ _ _ _ _ Hhc Hha); assumption.
+            - simpl.
+              refine (perm_trans _ (Permutation_app (Permutation_refl _) H4)).
+              refine (perm_trans (Permutation_app_comm _ _) _).
+              rewrite app_assoc. apply Permutation_refl. }
+          { inv Hec. simpl. exact (priqueue_elems_cons _ _ _ _ _ H1 H2 H4). }
+      * inv Hpq. inv Heq. destruct t.
+          { refine (priqueue_elems_cons _ _ _ _ _ Hec _ _).
+            - destruct H as [H | Hht]; [discriminate H|].
+              refine (IHp _ _ _ Hpp H0 (or_intror _) _ _ _ H2 H7 _).
+              + apply smash_valid; assumption.
+              + apply (smash_elems _ _ _ _ _ Hha Hht H1 H6).
+            - apply (Permutation_app (Permutation_refl _)).
+              refine (perm_trans _ (Permutation_app H4 H9)).
+              rewrite <- app_assoc. rewrite <- app_assoc.
+              apply (Permutation_app (Permutation_refl _)).
+              rewrite app_assoc. rewrite app_assoc.
+              apply (Permutation_app (Permutation_app_comm _ _) (Permutation_refl _)). }
+          { inv H6. simpl in H9.
+            pose proof (fun c ce Hhc Hec => IHp _ c _ Hpp H0 Hhc _ _ ce H2 H7 Hec) as IH.
+            destruct c.
+            - destruct Hhc as [Hhc | Hhc]; [discriminate Hhc|].
+              refine (priqueue_elems_cons _ _ _ ((ce ++ hl) ++ tl ++ tl0) _ tree_elems_leaf _ _).
+              + apply IH.
+                * right. apply smash_valid; assumption.
+                * apply (smash_elems _ _ _ _ _ Hhc Hha); assumption.
+              + simpl. rewrite <- app_assoc.
+                apply (Permutation_app (Permutation_refl _)).
+                rewrite app_assoc. apply (Permutation_app H4 H9).
+            - inv Hec. simpl.
+              refine (priqueue_elems_cons _ _ _ ([] ++ tl ++ tl0) _ H1 _ _).
+              + apply IH.
+                * left. reflexivity.
+                * apply tree_elems_leaf.
+              + simpl. rewrite app_assoc. apply (Permutation_app H4 H9). }
+    + inv Hep. inv H1. simpl in H4. destruct q.
+      * inv Heq. rewrite app_nil_r.
+        apply (priqueue_elems_cons _ _ _ _ _ Hec H2).
+        apply (Permutation_app (Permutation_refl _) H4).
+      * inv Heq. simpl in Hpq. destruct Hpq as [Hht Hpq].
+        pose proof (fun c ce Hhc Hec => IHp _ c _ Hpp Hpq Hhc _ _ ce H2 H3 Hec) as IH.
+        destruct t.
+          { destruct Hht as [Hht | Hht]; [discriminate Hht|].
+            destruct c.
+            - destruct Hhc as [Hhc | Hhc]; [discriminate Hhc|].
+              refine (priqueue_elems_cons _ _ _ ((ce ++ hl) ++ tl ++ tl0) _ tree_elems_leaf _ _).
+              + apply IH.
+                * right. apply smash_valid; assumption.
+                * apply (smash_elems _ _ _ _ _ Hhc Hht); assumption.
+              + simpl. rewrite <- app_assoc.
+                apply (Permutation_app (Permutation_refl _)).
+                apply (perm_trans (Permutation_app_comm _ _)).
+                rewrite <- app_assoc.
+                exact (Permutation_app H4 (perm_trans (Permutation_app_comm _ _) H6)).
+            - inv Hec. simpl. refine (priqueue_elems_cons _ _ _ ([] ++ tl ++ tl0) _ H1 _ _).
+              + apply IH.
+                * left. reflexivity.
+                * apply tree_elems_leaf.
+              + simpl. refine (perm_trans _ (Permutation_app H4 H6)).
+                rewrite app_assoc. rewrite app_assoc.
+                refine (Permutation_app (Permutation_app_comm _ _) (Permutation_refl _)). }
+          { inv H1. simpl in H6.
+            refine (priqueue_elems_cons _ _ _ ([] ++ tl ++ tl0) _ Hec _ _).
+            + apply IH.
+              * left. reflexivity.
+              * apply tree_elems_leaf.
+            + simpl. apply (Permutation_app (Permutation_refl _)).
+              apply (Permutation_app H4 H6). }
+Qed.
 (** [] *)
 
 (** **** Exercise: 2 stars, standard, optional (merge_relate) *)
@@ -359,14 +683,241 @@ Theorem merge_relate:
        Abs p pl -> Abs q ql -> Abs (merge p q) al ->
        Permutation al (pl++ql).
 Proof.
-(* FILL IN HERE *) Admitted.
+  intros p q pl ql al Hpp Hpq Hep Heq Hea.
+  apply (abs_perm (merge p q)).
+  - apply merge_priq; assumption.
+  - exact Hea.
+  - unfold merge. change (pl ++ ql) with ([] ++ pl ++ ql).
+    apply (join_elems _ _ _ _ Hpp Hpq).
+    + left. reflexivity.
+    + assumption.
+    + assumption.
+    + apply tree_elems_leaf.
+Qed.
 (** [] *)
+
 
 (** **** Exercise: 5 stars, standard, optional (delete_max_None_relate) *)
 Theorem delete_max_None_relate:
         forall p, priq p -> (Abs p nil <-> delete_max p = None).
-(* FILL IN HERE *) Admitted.
+Proof.
+  intros q Hpq. split.
+  - assert (perm_nil_eq : forall (l1 l2 : list key), Permutation (l1 ++ l2) [] -> l1 = [] /\ l2 = []).
+      { intros l1 l2 H. apply Permutation_sym in H.
+        apply Permutation_nil in H. apply app_eq_nil in H. exact H. }
+    assert (H: forall q n, priq' n q -> Abs q [] -> find_max q = None).
+      { induction q0; intros n Hp He.
+        - reflexivity.
+        - simpl in *. destruct Hp as [Ha Hq0].
+          inv He.
+          apply perm_nil_eq in H4. destruct H4. subst hl tl.
+          destruct a.
+          + inv H1. apply Permutation_nil in H7. discriminate H7.
+          + exact (IHq0 _ Hq0 H2). }
+    intros Hq. unfold delete_max.
+    rewrite (H _ _ Hpq Hq). reflexivity.
+  - intros Hd. unfold delete_max in Hd.
+    destruct (find_max q) eqn:Ef.
+    + destruct (delete_max_aux k q). discriminate Hd.
+    + clear Hd.
+      assert (H : forall q n, priq' n q -> find_max q = None -> Abs q []).
+        { induction q0; intros n Hp Hf.
+          - apply priqueue_elems_nil.
+          - simpl in Hp. destruct Hp as [Ha Hq0].
+            simpl in Hf. destruct a; [discriminate Hf|].
+            exact (priqueue_elems_cons _ _ _ _ _ tree_elems_leaf (IHq0 _ Hq0 Hf) (Permutation_refl _)). }
+      exact (H _ _ Hpq Ef).
+Qed.
 (** [] *)
+
+
+Lemma tree_elems_releate : forall t n m tl,
+  pow2heap' n m t ->
+  tree_elems t tl ->
+  Forall (ge m) tl.
+Proof.
+  intros t n m tl H He. generalize dependent m. generalize dependent n.
+  induction He; intros n m Hp.
+  - apply Forall_nil.
+  - destruct n; [contradiction Hp|]. simpl in Hp.
+    destruct Hp as [Hm [Hpl Hpr]].
+    apply (Permutation_Forall (Permutation_sym H)).
+    apply (Forall_cons _ Hm). apply Forall_app. split.
+    + refine (Forall_impl _ _ (IHHe1 _ _ Hpl)). lia.
+    + exact (IHHe2 _ _ Hpr).
+Qed.
+
+
+Lemma find_max'_relate : forall p n pl,
+  priq' n p ->
+  Abs p pl ->
+  forall c k,
+  find_max' c p = k ->
+  k >= c /\ Forall (ge k) pl /\ (k = c \/ In k pl).
+Proof.
+  induction p; intros n pl Hp He c k Hf.
+  - inv He. simpl. split.
+    + lia.
+    + exact (conj (Forall_nil _) (or_introl eq_refl)).
+  - simpl in *. destruct Hp as [Ha Hp]. inv He.
+    destruct a.
+    + destruct Ha as [Ha | Ha]; [discriminate Ha|].
+      specialize (IHp _ _ Hp H2).
+      simpl in Ha. destruct a2; [contradiction Ha|].
+      inv H1. inv H7. rewrite app_nil_r in H8. apply Permutation_sym in H8.
+      assert (Forall (ge k) hl) as Hghl.
+        { apply (Permutation_Forall H8). apply Forall_cons.
+          - apply Nat.le_refl.
+          - exact (tree_elems_releate _ _ _ _ Ha H5). }
+
+      specialize (tree_elems_releate _ _ _ _ Ha H5) as Hgb.
+      bdestruct (k >? c).
+      * destruct (IHp k _ eq_refl) as [Hg [Hf Hc]].
+        split; [| split].
+          { lia. }
+          { apply (Permutation_Forall H4). apply Forall_app. split.
+            - apply (@Forall_impl _ (ge k)).
+              + lia.
+              + exact Hghl.
+            - exact Hf. }
+          { right. apply (Permutation_in _ H4). apply in_or_app.
+            destruct Hc.
+            - left. rewrite H0.
+              apply (Permutation_in _ H8). simpl.
+              left. reflexivity.
+            - right. exact H0. }
+      * destruct (IHp c _ eq_refl) as [Hg [Hf Hc]].
+        refine (conj Hg (conj _ _)).
+          { apply (Permutation_Forall H4). apply Forall_app. split.
+            - apply (@Forall_impl _ (ge k)).
+              + lia.
+              + exact Hghl.
+            - exact Hf. }
+          { destruct Hc as [Hcc | Hci].
+            - left. exact Hcc.
+            - right. apply (Permutation_in _ H4). apply in_or_app.
+              right. exact Hci. }
+    + inv H1. simpl in H4. apply (priqueue_elems_ext _ _ _ H4) in H2.
+      exact (IHp _ _ Hp H2 _ _ eq_refl).
+Qed.
+
+Lemma find_max_Some_relate : forall p n k pl,
+  priq' n p ->
+  find_max p = Some k ->
+  Abs p pl ->
+  Forall (ge k) pl /\ In k pl.
+Proof.
+  induction p; intros n k pl Hpp Hf Hep.
+  - discriminate Hf.
+  - simpl in *. destruct Hpp as [Hha Hpp].
+    destruct a.
+    + injection Hf as Hf.
+      inv Hep.
+      destruct Hha as [Hha | Hha]; [discriminate Hha|]. simpl in Hha.
+      destruct a2; [contradiction Hha|].
+      destruct (find_max'_relate _ _ _ Hpp H2 k0 _ eq_refl) as [Hg [Hf Hi]].
+      inv H1. inv H7. rewrite app_nil_r in H8.
+      split.
+      * apply (Permutation_Forall H4). apply Forall_app. split.
+          { apply (@Forall_impl _ (ge k0)).
+            - lia.
+            - apply (Permutation_Forall (Permutation_sym H8)).
+              apply Forall_cons.
+              + apply Nat.le_refl.
+              + exact (tree_elems_releate _ _ _ _ Hha H5). }
+          { exact Hf. }
+      * apply (Permutation_in _ H4). apply in_or_app.
+        destruct Hi as [Hik | Hit].
+          { left. apply (Permutation_in _ (Permutation_sym H8)). left.
+            symmetry. exact Hik. }
+          { right. exact Hit. }
+    + refine (IHp _ _ _ Hpp Hf _).
+      inv Hep. inv H1. simpl in *. exact (priqueue_elems_ext _ _ _ H4 H2).
+Qed.
+
+Lemma unzip_elem : forall t cont k n tl cl,
+  pow2heap' n k t ->
+  Abs (cont nil) cl ->
+  tree_elems t tl ->
+  Abs (unzip t cont) (tl ++ cl).
+Proof.
+  induction t; intros cont tk n tl cl Hp Hec Het.
+  - destruct n; [contradiction Hp|]. simpl in *.
+    destruct Hp as [Hk [Hpt1 Hpt2]].
+    inv Het. apply (priqueue_elems_ext _ (br ++ (k :: bl ++ cl))).
+    + change (k :: bl ++ cl) with ((k::bl) ++ cl). rewrite app_assoc.
+      refine (Permutation_app (perm_trans _ (Permutation_sym H5)) (Permutation_refl _)).
+      apply Permutation_sym. apply Permutation_cons_app. apply Permutation_app_comm.
+    + apply (IHt2 _ _ _ _ _ Hpt2).
+      * change (k :: bl ++ cl) with ((k::bl) ++ cl).
+        refine (priqueue_elems_cons _ _ _ _ _ _ Hec (Permutation_refl _)).
+        apply (tree_elems_node _ _ _ _ _ _ H2 tree_elems_leaf).
+        rewrite app_nil_r. apply Permutation_refl.
+      * assumption.
+  - inv Het. simpl. assumption. 
+Qed.
+
+Lemma delete_max_aux_relate : forall p n k pl,
+  priq' n p ->
+  Abs p pl ->
+  Forall (ge k) pl ->
+  In k pl ->
+  let (p0,p1) := delete_max_aux k p in
+  forall p0l p1l,
+    Abs p0 p0l ->
+    Abs p1 p1l ->
+    Permutation pl (k :: p0l ++ p1l).
+Proof.
+  induction p; intros n k pl Hpp Hep Hgk Hik.
+  - inv Hep. contradiction Hik.
+  - simpl in *. destruct Hpp as [Ha Hpp].
+    inv Hep. destruct a as [ak al ar|].
+    + destruct Ha as [Ha | Ha]; [discriminate Ha|]. simpl in Ha.
+      destruct ar; [contradiction Ha|].
+      
+      apply (Permutation_Forall (Permutation_sym H4)) in Hgk.
+      apply Forall_app in Hgk. destruct Hgk as [Hgh Hgt].
+      apply (Permutation_in _ (Permutation_sym H4)) in Hik.
+      apply in_app_or in Hik.
+
+      bdestruct (k >? ak).
+      * assert (In k tl).
+          { destruct Hik; [| assumption]. exfalso.
+            inv H1. inv H9. rewrite app_nil_r in H10.
+            apply (Permutation_Forall H10) in Hgh.
+            apply (Permutation_in _ H10) in H0. simpl in H0.
+            destruct H0; [lia|].
+            apply (tree_elems_releate _ _ _ _ Ha) in H7.
+            rewrite Forall_forall in H7. apply H7 in H0.
+            lia. }
+        specialize (IHp _ _ _ Hpp H2 Hgt H0).
+        destruct (delete_max_aux k p) as [pr pk]. intros p0l p1l Hep0 Hep1.
+        inv Hep0. apply (perm_trans (Permutation_sym H4)).
+        apply (perm_trans (Permutation_app (tree_perm _ _ _ H1 H6) (IHp _ _ H7 Hep1))).
+        apply Permutation_sym. apply Permutation_cons_app.
+        rewrite app_assoc. exact (Permutation_app (Permutation_sym H9) (Permutation_refl _)).
+      * inv H1. inv H8. rewrite app_nil_r in H9.
+        assert (k = ak).
+          { specialize (Permutation_in ak (Permutation_sym H9) (or_introl eq_refl)) as Hi.
+            rewrite Forall_forall in Hgh. apply Hgh in Hi.
+            lia. }
+        subst ak. intros p0l p1l Hep0 Hep1.
+        apply (perm_trans (Permutation_sym H4)).
+        apply (perm_trans (Permutation_app H9 (Permutation_refl _))). simpl.
+        apply perm_skip. apply (perm_trans (Permutation_app_comm _ _)).
+        apply Permutation_app.
+          { inv Hep0. inv H3. simpl in *. refine (perm_trans _ H8).
+            apply (abs_perm' p); assumption. }
+          { specialize (unzip_elem _ (fun u => u) _ _ _ _ Ha priqueue_elems_nil H6) as Heu.
+            rewrite app_nil_r in Heu.
+            exact (abs_perm' _ _ _ Heu Hep1). }
+    + inv H1. simpl in *.
+      apply (priqueue_elems_ext _ _ _ H4) in H2.
+      specialize (IHp _ _ _ Hpp H2 Hgk Hik). destruct (delete_max_aux k p).
+      intros p0l p1l Hep0 Hep1. apply IHp.
+      * inv Hep0. inv H1. simpl in *. apply (priqueue_elems_ext _ _ _ H6 H3).
+      * assumption.
+Qed.
 
 (** **** Exercise: 5 stars, standard, optional (delete_max_Some_relate) *)
 Theorem delete_max_Some_relate:
@@ -375,7 +926,34 @@ Theorem delete_max_Some_relate:
    delete_max p = Some (k,q) ->
    Abs q ql ->
    Permutation pl (k::ql) /\ Forall (ge k) ql.
-(* FILL IN HERE *) Admitted.
+Proof.
+  intros p q k pl ql Hp Hep Hd Heq. unfold delete_max in Hd.
+  destruct (find_max p) eqn:Ef; [| discriminate Hd].
+  destruct (find_max_Some_relate _ _ _ _ Hp Ef Hep) as [Hgk Hik].
+  specialize (delete_max_aux_relate _ _ _ _ Hp Hep Hgk Hik) as Hda.
+  specialize (delete_max_aux_priq k0 _ _ Hp) as Hpd.
+  destruct (delete_max_aux k0 p). injection Hd as E0 E1. subst k q.
+  assert (Permutation pl (k0 :: ql)).
+    { destruct Hpd as [Hpp0 Hpp1].
+      destruct (can_relate p0 Hpp0) as [p0l Hep0].
+      destruct (can_relate p1 Hpp1) as [p1l Hep1].
+      specialize (Hda _ _ Hep0 Hep1).
+      apply (perm_trans Hda). apply perm_skip.
+      apply (abs_perm (join p0 p1 Leaf)).
+      + exact (join_valid _ _ _ _ Hpp0 Hpp1 (or_introl eq_refl)).
+      + change (p0l ++ p1l) with ([] ++ p0l ++ p1l).
+        apply join_elems with (n := 0).
+        * assumption.
+        * assumption.
+        * left. reflexivity.
+        * assumption.
+        * assumption.
+        * apply tree_elems_leaf.
+      + assumption. }
+  split.
+  - exact H.
+  - apply Forall_inv_tail with k0. exact (Permutation_Forall H Hgk).
+Qed.
 (** [] *)
 
 (** With the following line, we're done!  We have demonstrated that
